

1 Derivative

1.1

Given:

$$f(x) = \frac{1}{\ln(1+x)} - \frac{1}{x}, \quad x \in [0, 1], \quad \lambda = \max_{x \in [0, 1]} f(x), \quad \mu = \min_{x \in [0, 1]} f(x)$$

As $x \rightarrow 0^+$:

$$\ln(1+x) = x - \frac{x^2}{2} + O(x^3)$$

$$\frac{1}{\ln(1+x)} = \frac{1}{x} \cdot \frac{1}{1 - \frac{x}{2} + O(x^2)} = \frac{1}{x} \left(1 + \frac{x}{2} + O(x^2)\right) = \frac{1}{x} + \frac{1}{2} + O(x)$$

$$f(x) = \left(\frac{1}{x} + \frac{1}{2}\right) - \frac{1}{x} + O(x) = \frac{1}{2} + O(x) \rightarrow \frac{1}{2}$$

At $x = 1$:

$$f(1) = \frac{1}{\ln 2} - 1$$

The derivative is:

$$f'(x) = -\frac{1}{(1+x)\ln^2(1+x)} + \frac{1}{x^2}$$

Setting $f'(x) = 0$ gives:

$$\frac{1}{x^2} = \frac{1}{(1+x)\ln^2(1+x)} \Rightarrow (1+x)\ln^2(1+x) = x^2$$

Numerical analysis shows $f'(x) < 0$ on $[0, 1]$, so $f(x)$ is strictly decreasing. Therefore:

$$\lambda = \lim_{x \rightarrow 0^+} f(x) = \frac{1}{2}, \quad \mu = f(1) = \frac{1}{\ln 2} - 1$$

1.2

Given $f(x)$ has continuous second-order derivatives on $[a, b]$. Prove:

$$\lim_{n \rightarrow \infty} n^2 \left[\int_a^b f(x) dx - \frac{b-a}{n} \sum_{k=1}^n f\left(a + \frac{2k-1}{2n}(b-a)\right) \right] = \frac{(b-a)^2}{24} [f'(b) - f'(a)]$$

Proof: Consider the error for one subinterval $[x_{k-1}, x_k]$ where $x_k = a + \frac{k}{n}(b-a)$ and midpoint $c_k = a + \frac{2k-1}{2n}(b-a)$. By Taylor expansion around c_k :

$$f(x) = f(c_k) + f'(c_k)(x - c_k) + \frac{f''(\xi_k)}{2}(x - c_k)^2$$
$$\int_{x_{k-1}}^{x_k} f(x) dx = f(c_k)h + \frac{f''(\eta_k)}{24}h^3$$

where $h = \frac{b-a}{n}$.

Summing over all subintervals:

$$\int_a^b f(x) dx - \frac{b-a}{n} \sum_{k=1}^n f(c_k) = \sum_{k=1}^n \frac{f''(\eta_k)}{24} h^3 = \frac{(b-a)^3}{24n^2} \cdot \frac{1}{n} \sum_{k=1}^n f''(\eta_k)$$

As $n \rightarrow \infty$, $\frac{1}{n} \sum_{k=1}^n f''(\eta_k) \rightarrow \frac{1}{b-a} \int_a^b f''(x) dx = \frac{f'(b) - f'(a)}{b-a}$. Therefore:

$$\lim_{n \rightarrow \infty} n^2 \left[\int_a^b f(x) dx - \frac{b-a}{n} \sum_{k=1}^n f(c_k) \right] = \frac{(b-a)^2}{24} [f'(b) - f'(a)]$$

2 Limits

2.1

Compute:

$$I = \lim_{x \rightarrow 0} \frac{\ln(\cos x)}{x^2}$$

Using Taylor expansion:

$$\begin{aligned}\cos x &= 1 - \frac{x^2}{2} + O(x^4) \\ \ln(\cos x) &= \ln\left(1 - \frac{x^2}{2} + O(x^4)\right) = -\frac{x^2}{2} + O(x^4) \\ I &= \lim_{x \rightarrow 0} \frac{-\frac{x^2}{2} + O(x^4)}{x^2} = -\frac{1}{2}\end{aligned}$$

2.2

Compute:

$$I = \lim_{x \rightarrow 0} \frac{\ln(\cos x + x \sin 2x)}{e^{x^2} - \sqrt[3]{1 - x^2}}$$

Expand numerator:

$$\begin{aligned}\cos x &= 1 - \frac{x^2}{2} + O(x^4) \\ x \sin 2x &= 2x^2 - \frac{4}{3}x^4 + O(x^6) \\ \cos x + x \sin 2x &= 1 + \frac{3}{2}x^2 + O(x^4) \\ \ln(\cos x + x \sin 2x) &= \frac{3}{2}x^2 + O(x^4)\end{aligned}$$

Expand denominator:

$$\begin{aligned}e^{x^2} &= 1 + x^2 + O(x^4) \\ \sqrt[3]{1 - x^2} &= 1 - \frac{1}{3}x^2 + O(x^4) \\ e^{x^2} - \sqrt[3]{1 - x^2} &= \frac{4}{3}x^2 + O(x^4)\end{aligned}$$

Therefore:

$$I = \lim_{x \rightarrow 0} \frac{\frac{3}{2}x^2 + O(x^4)}{\frac{4}{3}x^2 + O(x^4)} = \frac{3/2}{4/3} = \frac{9}{8}$$

3 Integrals

3.1

$$I = \int \sec x dx$$

Multiply numerator and denominator by $\sec x + \tan x$:

$$I = \int \frac{\sec x(\sec x + \tan x)}{\sec x + \tan x} dx = \int \frac{\sec^2 x + \sec x \tan x}{\sec x + \tan x} dx$$

Let $u = \sec x + \tan x$, then $du = (\sec x \tan x + \sec^2 x) dx$:

$$I = \int \frac{du}{u} = \ln |u| + C = \ln |\sec x + \tan x| + C$$

3.2

$$I = \int \frac{dx}{x^2 + a^2}$$

Let $x = a \tan t$, $dx = a \sec^2 t dt$:

$$I = \int \frac{a \sec^2 t}{a^2(\tan^2 t + 1)} dt = \frac{1}{a} \int dt = \frac{1}{a} t + C = \frac{1}{a} \arctan\left(\frac{x}{a}\right) + C$$

3.3

$$I = \int \frac{dx}{\sqrt{x^2 + a^2}}$$

Let $x = a \tan t$, $dx = a \sec^2 t dt$, $\sqrt{x^2 + a^2} = a \sec t$:

$$I = \int \frac{a \sec^2 t}{a \sec t} dt = \int \sec t dt = \ln |\sec t + \tan t| + C$$

Substitute back: $\sec t = \frac{\sqrt{x^2 + a^2}}{a}$, $\tan t = \frac{x}{a}$:

$$I = \ln \left| \frac{x}{a} + \frac{\sqrt{x^2 + a^2}}{a} \right| + C = \ln \left| x + \sqrt{x^2 + a^2} \right| + C'$$

4 Multiple Integrals

4.1

$$D = \{(x, y) \mid x^2 + y^2 \leq \pi\}, \quad I = \iint_D \left(\sin(x^2) \cos(y^2) + x\sqrt{x^2 + y^2} \right) dx dy$$

The second term $x\sqrt{x^2 + y^2}$ is odd in x , so its integral over the symmetric domain D is zero. Thus:

$$I = \iint_D \sin(x^2) \cos(y^2) dx dy$$

Using the identity:

$$\sin(x^2) \cos(y^2) = \frac{1}{2} [\sin(x^2 + y^2) + \sin(x^2 - y^2)]$$

The $\sin(x^2 - y^2)$ term integrates to zero due to symmetry. Use polar coordinates:

$$\begin{aligned} x &= r \cos \theta, & y &= r \sin \theta \\ I &= \frac{1}{2} \int_0^{2\pi} \int_0^{\sqrt{\pi}} \sin(r^2) \cdot r dr d\theta \\ &= \pi \int_0^{\sqrt{\pi}} \sin(r^2) r dr \end{aligned}$$

Let $u = r^2$, $du = 2r dr$:

$$I = \pi \int_0^{\pi} \sin u \cdot \frac{du}{2} = \frac{\pi}{2} [-\cos u]_0^{\pi} = \frac{\pi}{2} (1 - (-1)) = \pi$$

4.2

$$I = \iiint_S (x^2 - x) dy dz + (y^2 - y) dz dx + (z^2 - z) dx dy$$

where S is the upper side of the upper hemisphere $x^2 + y^2 + z^2 = R^2$ ($z \geq 0$).

Use spherical coordinates:

$$\begin{aligned} x &= r \sin \theta \cos \phi, & y &= r \sin \theta \sin \phi, & z &= r \cos \theta \\ 0 &\leq r \leq R, & 0 &\leq \theta \leq \frac{\pi}{2}, & 0 &\leq \phi \leq 2\pi \end{aligned}$$

$$\begin{aligned} I &= \int_0^{2\pi} \int_0^{\pi/2} \int_0^R (2r \cos \theta - 3) r^2 \sin \theta dr d\theta d\phi \\ &= 2\pi \int_0^{\pi/2} \int_0^R (2r^3 \cos \theta - 3r^2) \sin \theta dr d\theta \\ &= 2\pi \int_0^{\pi/2} \left(\frac{R^4}{2} \cos \theta - R^3 \right) \sin \theta d\theta \\ &= 2\pi \left[-\frac{R^4}{4} \cos^2 \theta + R^3 \cos \theta \right]_0^{\pi/2} \\ &= 2\pi \left(\frac{R^4}{4} - R^3 \right) = \frac{\pi R^4}{2} - 2\pi R^3 \end{aligned}$$